

# Full Newton Hessian for Frequency-Domain Maxwell Inversion

## 1 Frequency-Domain Maxwell Equations

Assume time convention  $e^{-i\omega t}$ .

$$\nabla \times \mathbf{E} = i\omega \mathbf{B}, \quad (1)$$

$$\nabla \times \mathbf{H} = \mathbf{J}_s + \sigma \mathbf{E} - i\omega \varepsilon \mathbf{E}, \quad (2)$$

$$\mathbf{B} = \mu \mathbf{H}. \quad (3)$$

Eliminate  $\mathbf{H}$  and  $\mathbf{B}$ :

$$\mathbf{H} = \mu^{-1} \mathbf{B} = \mu^{-1} (1/i\omega) \nabla \times \mathbf{E}.$$

Substitute into Ampère's law:

$$\nabla \times (\mu^{-1} \nabla \times \mathbf{E}) - i\omega \sigma \mathbf{E} - \omega^2 \varepsilon \mathbf{E} = \mathbf{f}.$$

Define forward operator:

$$\mathcal{A}(m) \mathbf{E} = \mathbf{f}, \quad m = (\sigma, \varepsilon, \mu).$$

## 2 Misfit Functional

$$J(m) = \frac{1}{2} \|\mathbf{P} \mathcal{A}(m) - \mathbf{d}\|^2.$$

## 3 First-Order Linearization

Let

$$m \rightarrow m + \delta m, \quad \mathbf{E} \rightarrow \mathbf{E} + \delta \mathbf{E}.$$

Linearize forward equation:

$$\mathcal{A}(m + \delta m)(\mathbf{E} + \delta \mathbf{E}) = \mathbf{f}.$$

Expand:

$$\mathcal{A}(m) \mathbf{E} + \mathcal{A}(m) \delta \mathbf{E} + D_m \mathcal{A}[\delta m] \mathbf{E} = \mathbf{f}.$$

Subtract original equation:

$$\mathcal{A}(m)\delta\mathbf{E} = -D_m\mathcal{A}[\delta m]\mathbf{E}.$$

Thus,

$$\delta\mathbf{E} = -\mathcal{A}^{-1}D_m\mathcal{A}[\delta m]\mathbf{E}.$$

## 4 Fréchet Derivatives

### 4.1 Derivative w.r.t. $\sigma$

$$D_\sigma\mathcal{A}[\delta\sigma]\mathbf{E} = i\omega\delta\sigma\mathbf{E}.$$

### 4.2 Derivative w.r.t. $\varepsilon$

$$D_\varepsilon\mathcal{A}[\delta\varepsilon]\mathbf{E} = \omega^2\delta\varepsilon\mathbf{E}.$$

### 4.3 Derivative w.r.t. $\mu$

Use

$$\delta(\mu^{-1}) = -\mu^{-2}\delta\mu.$$

Then

$$D_\mu\mathcal{A}[\delta\mu]\mathbf{E} = -\nabla \times (\mu^{-2}\delta\mu\nabla \times \mathbf{E}).$$

## 5 Adjoint Equation

Define Lagrangian:

$$\mathcal{L} = J(m) + \Re\langle \mathbf{\Lambda}, \mathcal{A}\mathbf{E} - \mathbf{f} \rangle.$$

Variation w.r.t.  $\mathbf{E}$ :

$$\delta\mathcal{L} = \langle \mathbf{P}^*(\mathbf{P}\mathbf{E} - \mathbf{d}), \delta\mathbf{E} \rangle + \langle \mathbf{\Lambda}, \mathcal{A}\delta\mathbf{E} \rangle.$$

Thus adjoint equation:

$$\mathcal{A}^\dagger\mathbf{\Lambda} = \mathbf{P}^*(\mathbf{P}\mathbf{E} - \mathbf{d}).$$

Explicit form:

$$\nabla \times (\mu^{-1}\nabla \times \mathbf{\Lambda}) + i\omega\sigma\mathbf{\Lambda} - \omega^2\varepsilon\mathbf{\Lambda} = \mathbf{q}.$$

## 6 Gradient

$$\delta J = -\Re\langle \mathbf{\Lambda}, D_m\mathcal{A}[\delta m]\mathbf{E} \rangle.$$

## 6.1 Conductivity

$$\nabla_{\sigma} J = -\Re(i\omega \mathbf{\Lambda} \cdot \mathbf{E}).$$

## 6.2 Permittivity

$$\nabla_{\varepsilon} J = -\Re(\omega^2 \mathbf{\Lambda} \cdot \mathbf{E}).$$

## 6.3 Permeability

Using integration by parts:

$$\nabla_{\mu} J = \Re \left( \mu^{-2} (\nabla \times \mathbf{E}) \cdot (\nabla \times \mathbf{\Lambda}) \right).$$

## 7 Gauss–Newton Hessian

Jacobian:

$$\mathcal{J} = -\mathbf{P} \mathcal{A}^{-1} D_m \mathcal{A}.$$

Gauss–Newton approximation:

$$H_{GN} = \mathcal{J}^* \mathcal{J}.$$

## 8 Full Newton Hessian

Now include second-order field derivatives.

Second variation:

$$\delta^2 \mathbf{E} = -\mathcal{A}^{-1} \left( D_m^2 \mathcal{A}[\delta m_1, \delta m_2] \mathbf{E} + D_m \mathcal{A}[\delta m_1] \delta \mathbf{E}_2 + D_m \mathcal{A}[\delta m_2] \delta \mathbf{E}_1 \right).$$

Full Hessian:

$$H_{Newton} = H_{GN} + H_{2nd}.$$

Second-order term:

$$H_{2nd} = \langle \mathbf{\Lambda}, D_m^2 \mathcal{A}[\cdot, \cdot] \mathbf{E} \rangle.$$

## 9 Explicit Second Derivatives

### 9.1 $\sigma$

Since linear:

$$D_{\sigma}^2 \mathcal{A} = 0.$$

### 9.2 $\varepsilon$

$$D_{\varepsilon}^2 \mathcal{A} = 0.$$

### 9.3 $\mu$

$$\delta^2(\mu^{-1}) = 2\mu^{-3}(\delta\mu_1)(\delta\mu_2).$$

Thus

$$D_\mu^2 \mathcal{A} = 2\nabla \times (\mu^{-3} \delta\mu_1 \delta\mu_2 \nabla \times \mathbf{E}).$$

## 10 Final Newton Hessian Expression

$$H_{Newton} = \mathcal{J}^* \mathcal{J} + \Re \langle \mathbf{\Lambda}, D_m^2 \mathcal{A} \mathbf{E} \rangle.$$

Only  $\mu$  contributes to second-order term.